src/association_list.v
@@ -2,7 +2,12 @@ Require Import List Nat Arith String.
 Import ListNotations.
 Require Import Mmx.ast_instructions.
 
-  
+(*
+Variable tag : Type.
+Variable beq_T : tag -> tag -> bool.
+Variable beq_T_refl : forall (t : tag), beq_T t t = true.
+Variable beq_T_rev : forall (t1 t2 : tag), beq_T t1 t2 = true <-> t1 = t2.
+*)
 (*=assoc *)
 Definition assoc : Type :=
   tag * nat.
@@ -38,7 +43,7 @@ Fixpoint lookdown (n : nat) (l : tag_opcode_assoc) : option tag :=
 
 (* this table is an association list of type tag_opcode_assoc with every associations that can be made in our langage *)
 (*=encdec *)
-Variable encdec : tag_opcode_assoc.
+Definition encdec := [(bidon1, 0); (bidon2, 1)]. (*tag_opcode_assoc.*)
 Variable forall_tag : (tag -> bool) -> bool.
 Variable forall_tag_spec1 : forall (f : tag -> bool), (forall (t: tag), f t = true) -> forall_tag f = true.
 Variable forall_tag_spec2 : forall (f : tag -> bool), forall_tag f = true -> (forall (t: tag), f t = true).
